commenting

src/tls/ConnInvariant.fst
@@ -8,13 +8,28 @@ module MM = MonotoneMap
 module MR = FStar.Monotonic.RRef
 module HH = FStar.HyperHeap
 module MS = MasterSecret
-module N = Nonce
-module I = IdNonce
+module N  = Nonce
+module I  = IdNonce
 module AE = StreamAE
 
 type id = StreamAE.id
-let r_conn (r:random) = c:connection{c.hs.nonce = r}
+//The type of connection with a particular nonce
+//   `r_conn n` should never really have more than 1 inhabitant, 
+//   one of the purposes of the conn_table defined below is to enforce that
+type r_conn (nonce:random) = c:connection{c.hs.nonce = nonce}
 
+//The connection associated with an id
+type i_conn (i:id) = r_conn (I.nonce_of_id i)
+
+(* -------------------------------------------------------------------------------- 
+   The nonce to connection table, defined in a few steps: 
+
+   1. The table is a partial map from (nonce:random) to (r_conn nonce)
+   
+   2. We have an `pairwise_disjoint` invariant on the 
+      table that connections associated with distinct nonces 
+      live in distinct regions. 
+  -------------------------------------------------------------------------------- *)
 let pairwise_disjoint (m:MM.map' random r_conn) = 
     forall r1 r2.{:pattern (is_Some (MM.sel m r1));
 		      (is_Some (MM.sel m r2))}
@@ -22,25 +37,41 @@ let pairwise_disjoint (m:MM.map' random r_conn) =
 	     ==> HH.disjoint (Some.v (MM.sel m r1)).region  
 		             (Some.v (MM.sel m r2)).region
 
-type conn_table_t = MM.t tls_tables_region random r_conn pairwise_disjoint
+type conn_tab_t = MM.t tls_tables_region random r_conn pairwise_disjoint
 
-let conn_table : conn_table_t = 
+let conn_tab : conn_tab_t = 
   MM.alloc #tls_tables_region #random #r_conn #pairwise_disjoint
 
-type ms_tab = MM.map' AE.id MS.writer 
-type c_tab  = MM.map' random r_conn 
+(*** MAIN STATEFUL INVARIANT ***)
+(* --------------------------------------------------------------------------------
+   We define a joint, stateful invariant to relate the contents 
+   of MasterSecret.ms_tab and conn_tab above.
 
+   The main application level invariant is:
+     Every writer in the ms_tab has an empty log
+     unless it has been registered within some epoch of a connection
+
+   To maintain this invariant, we strengthen it with some technical
+   nuances, mainly related to framing.
+  -------------------------------------------------------------------------------- *)
+
+//MS.ms_tab is a monontonic reference to an ms_t
+type ms_t = MM.map' AE.id MS.writer 
+
+//conn_tab is a monotonic reference to a c_t
+type c_t  = MM.map' random r_conn 
+
+//w is registered with c, in state h
 let registered (i:id{StAE.is_stream_ae i}) (w:StreamAE.writer i) (c:connection) (h:HH.t) = 
-  HH.disjoint (HS.region c.hs) tls_region /\
-  HH.contains_ref (HS.log c.hs) h /\
-  (exists e. SeqProperties.mem e  (HH.sel h (HS.log c.hs)) /\
-      (let i' = Handshake.hsId (Handshake.Epoch.h e) in
-        i=i' /\ StAE.stream_ae #i e.w == w))
-
-(* assume TLS_tables_region_color: color tls_tables_region = -1 *)
-
-let ms_conn_inv (ms:ms_tab)
- 		(conn:c_tab)
+  (exists e. SeqProperties.mem e  (HH.sel h (HS.log c.hs)) /\   //one of c's epochs, e
+      (let i' = Handshake.hsId (Handshake.Epoch.h e) in   //has an id corresponding to i
+        i=i' /\ StAE.stream_ae #i e.w == w))               //and holds w as as its writer
+  /\ HH.disjoint (HS.region c.hs) tls_region               //technical: TODO: we should have gotten this from the type of the connection, but seem to need it here
+  /\ HH.contains_ref (HS.log c.hs) h                       //technical: the heap contains c's handshake log
+	
+//The main invariant, relating an ms_tab and a conn_tab at index i, in state h
+let ms_conn_inv (ms:ms_t)
+ 		(conn:c_t)
 		(h:HyperHeap.t) 
 		(i:id) 
    = authId i /\ StAE.is_stream_ae i ==>  //Focused only on TLS-1.3 for now, hence the is_stream_ae guard
@@ -56,36 +87,51 @@ let ms_conn_inv (ms:ms_tab)
 	             (let copt = MM.sel conn (I.nonce_of_id i) in
   		      is_Some copt /\ registered i w (Some.v copt) h)))            //it's been registered with the connection associated with its nonce
 
-let ms_conn_invariant (ms:ms_tab)
- 		      (conn:c_tab)
+//The main invariant, for all AE.ids
+let ms_conn_invariant (ms:ms_t)
+ 		      (conn:c_t)
 		      (h:HyperHeap.t) 
   = forall (i:id) .{:pattern (MM.sel ms i)} ms_conn_inv ms conn h i
 
-let handshake_regions_exists (conn:c_tab) (h:HH.t) = 
+//A technical condition for framing: 
+//    Every handshake region exists in the current heap
+let handshake_regions_exists (conn:c_t) (h:HH.t) = 
   forall n.{:pattern (is_Some (MM.sel conn n))}
       is_Some (MM.sel conn n) 
        ==> (let hs_rgn = HS.region (C.hs (Some.v (MM.sel conn n))) in 
  	    Map.contains h hs_rgn /\
 	    HH.disjoint hs_rgn tls_tables_region)
 
+//Finally packaging it up as the main invariant:
 let mc_inv (h:HyperHeap.t) = 
-    HH.as_ref (MR.as_rref conn_table) =!= HH.as_ref (MR.as_rref MS.ms_tab)
-    /\ handshake_regions_exists (MR.m_sel h conn_table) h
-    /\ ms_conn_invariant (MR.m_sel h MS.ms_tab) (MR.m_sel h conn_table) h
+    HH.as_ref (MR.as_rref conn_tab) =!= HH.as_ref (MR.as_rref MS.ms_tab)     //Technical:the conn_tab and ms_tab are not aliased
+    /\ HH.contains_ref (MR.as_rref conn_tab) h                                //Technical:the heap contains the ms_tab
+    /\ HH.contains_ref (MR.as_rref MS.ms_tab) h                               //Technical:the heap contains the conn_tab
+    /\ handshake_regions_exists (MR.m_sel h conn_tab) h                       //Technical:every logged connection's handshake exists
+    /\ ms_conn_invariant (MR.m_sel h MS.ms_tab) (MR.m_sel h conn_tab) h       //Main joint stateful invariant
 
-//Checking the stability of the invariant
+(*** PROVING THE STABILITY OF mc_inv ***)
+(* --------------------------------------------------------------------------------
+   There are 4 main cases:
+     1. Deriving a new writer, using MS.derive 
+     2. Registering a writer with a connection
+     3. Mutating the log of some writer
+     4. Adding a new connection
+  -------------------------------------------------------------------------------- *)     
 
-//1. Deriving a new key involves adding a new writer to the ms table (because we tried a lookup at id and it failed)
-//   Easy: because a new log is empty and both cases of the conn table allow empty logs to be in ms
+(* 
+   Case 1:
+     Deriving a new key involves adding a new writer to the ms table (because we tried a lookup at id and it failed)
+     It's ok, because a new log is empty and adding an empty writer is fine regardless of the connections 
+*)
 val ms_derive_is_ok: h0:HyperHeap.t -> h1:HyperHeap.t -> i:AE.id -> w:MS.writer i 
   -> Lemma (requires 
-	        (let conn = MR.m_sel h0 conn_table in
+	        (let conn = MR.m_sel h0 conn_tab in
 	         let old_ms = MR.m_sel h0 MS.ms_tab in 
 		 let new_ms = MR.m_sel h1 MS.ms_tab in
-		 HH.contains_ref (MR.as_rref conn_table) h0 /\
-		 HH.contains_ref (MR.as_rref MS.ms_tab) h0  /\
-		 Map.contains h1 (StreamAE.State.region w)  /\
 		 mc_inv h0 /\ //we're initially in the invariant
+		 HH.contains_ref (MR.as_rref MS.ms_tab) h1  /\
+		 Map.contains h1 (StreamAE.State.region w)  /\
 		 is_epoch_rgn (StreamAE.State.region w) /\
 		 is_epoch_rgn (HH.parent (StreamAE.State.region w)) /\
 		 (* region_separated_from_all_handshakes (StreamAE.State.region w) conn /\         //the new writer is suitably separated from all handshakes *)
@@ -100,13 +146,12 @@ val ms_derive_is_ok: h0:HyperHeap.t -> h1:HyperHeap.t -> i:AE.id -> w:MS.writer 
 	 (ensures (mc_inv h1))
 let ms_derive_is_ok h0 h1 i w = 
   let aux :  j:id -> Lemma (let new_ms = MR.m_sel h1 MS.ms_tab in
-  			  let new_conn = MR.m_sel h1 conn_table in
+  			  let new_conn = MR.m_sel h1 conn_tab in
   			  ms_conn_inv new_ms new_conn h1 j) =
     fun j ->
       let old_ms = MR.m_sel h0 MS.ms_tab in 
       let new_ms = MR.m_sel h1 MS.ms_tab in
-      (* let new_conn = MR.m_sel h1 conn_table in *)
-      if (authId j && StAE.is_stream_ae j)
+      if authId j && StAE.is_stream_ae j
       then match MM.sel new_ms j with
            | None -> ()
            | Some ww ->
@@ -130,10 +175,11 @@ let try_ms_derive (epoch_region:rgn) (i:AE.id)
        (ensures (fun h0 w h1 -> 
 	   mc_inv h1))
   = let h0 = ST.get () in
-    MR.m_recall conn_table;
+    MR.m_recall conn_tab;
     MR.m_recall MS.ms_tab;
     let w = MasterSecret.derive epoch_region i in 
     MR.m_recall (AE.ilog (StreamAE.State.log w));
+    MR.m_recall MS.ms_tab;
     let h1 = ST.get () in 
     ms_derive_is_ok h0 h1 i w;
     w
@@ -166,17 +212,17 @@ let writer_region_within_connection
 val register_writer_in_epoch_ok: h0:HyperHeap.t -> h1:HyperHeap.t -> i:AE.id{authId i}
 		-> c:r_conn (I.nonce_of_id i) -> e:epoch (HS.region c.hs) (I.nonce_of_id i)
   -> Lemma (requires
-            (let ctab = MR.m_sel h0 conn_table in
+            (let ctab = MR.m_sel h0 conn_tab in
 	     let mstab = MR.m_sel h0 MS.ms_tab in
 	     let old_hs_log = HH.sel h0 (HS.log c.hs) in
      	     let new_hs_log = HH.sel h1 (HS.log c.hs) in
 	     let rgn = HS.region c.hs in
-	     HH.contains_ref (MR.as_rref conn_table) h0 /\
-	     HH.contains_ref (MR.as_rref MS.ms_tab) h0 /\
-	     HH.disjoint (HS.region c.hs) tls_region /\
+	     mc_inv h0 /\ //we're initially in the invariant
+	     (* HH.contains_ref (MR.as_rref conn_table) h0 /\ *)
+	     (* HH.contains_ref (MR.as_rref MS.ms_tab) h0 /\ *)
+	     (* HH.disjoint (HS.region c.hs) tls_region /\ *)
 	     HH.contains_ref (HS.log c.hs) h0 /\
 	     HH.contains_ref (HS.log c.hs) h1 /\
-	     mc_inv h0 /\ //we're initially in the invariant
 	     i=hsId (Epoch.h e) /\ //the epoch has id i
 	     (let w = StAE.stream_ae #i (Epoch.w e) in //the epoch writer
 	      let epochs = HH.sel h0 (HS.log c.hs) in
@@ -206,13 +252,13 @@ let register_writer_in_epoch_ok h0 h1 i c e =
      about the structure of the invariant.
   *)
   let aux :  j:id -> Lemma (let new_ms = MR.m_sel h1 MS.ms_tab in
-			   let new_conn = MR.m_sel h1 conn_table in
+			   let new_conn = MR.m_sel h1 conn_tab in
 			   ms_conn_inv new_ms new_conn h1 j) =
     fun j -> 			    
       let old_ms = MR.m_sel h0 MS.ms_tab in 
       let new_ms = MR.m_sel h1 MS.ms_tab in
-      let old_conn = MR.m_sel h0 conn_table in 
-      let new_conn = MR.m_sel h1 conn_table in
+      let old_conn = MR.m_sel h0 conn_tab in 
+      let new_conn = MR.m_sel h1 conn_tab in
       let old_hs_log = HH.sel h0 (HS.log c.hs) in
       let wi = StAE.stream_ae #i (Epoch.w e) in //the epoch writer
       let nonce = I.nonce_of_id i in
@@ -254,9 +300,9 @@ val mutate_registered_writer_ok : h0:HH.t -> h1:HH.t -> i:AE.id{authId i} -> w:M
 	       HH.modifies_one (StreamAE.State.region w) h0 h1 /\ //we modified at most the writer's region
 	       registered i w c h0 /\                             //the writer is registered in c
 	       MM.sel (MR.m_sel h0 MS.ms_tab) i = Some w   /\     //the writer is logged in the ms_tab
-	       MM.sel (MR.m_sel h0 conn_table) (I.nonce_of_id i) = Some c /\ //the connection is logged in the conn_table
-	       HH.contains_ref (MR.as_rref conn_table) h0 /\
-	       HH.contains_ref (MR.as_rref MS.ms_tab) h0 /\
+	       MM.sel (MR.m_sel h0 conn_tab) (I.nonce_of_id i) = Some c /\ //the connection is logged in the conn_table
+	       (* HH.contains_ref (MR.as_rref conn_tab) h0 /\ *)
+	       (* HH.contains_ref (MR.as_rref MS.ms_tab) h0 /\ *)
 	       HH.contains_ref (MR.as_rref (StreamAE.ilog (StreamAE.State.log w))) h1))
     (ensures (mc_inv h1)) 		 
 let mutate_registered_writer_ok h0 h1 i w c = ()
@@ -273,7 +319,6 @@ let mutate_registered_writer_ok h0 h1 i w c = ()
     qintro aux
 *)
 
-type i_conn (i:id) = r_conn (I.nonce_of_id i)
 //4. Adding a connection (writing to conn table) we note that none of the bad writers can be attributed to this connection
 //    -- So, we cannot be in the Some w, None case, as this is only for bad writers
 //    -- We cannot also be in the first case, since the conn table is monotonic and it doesn't already contain the id
@@ -287,13 +332,13 @@ let conn_hs_region_exists (c:connection) (h:HH.t) =
 val add_connection_ok: h0:HH.t -> h1:HH.t -> i:id -> c:i_conn i -> Lemma
   (requires (mc_inv h0 /\
 	     HH.modifies (Set.singleton tls_tables_region) h0 h1 /\
-	     HH.modifies_rref tls_tables_region !{HH.as_ref (MR.as_rref conn_table)} h0 h1 /\
-	     HH.contains_ref (MR.as_rref conn_table) h0 /\
-	     HH.contains_ref (MR.as_rref MS.ms_tab) h0 /\
+	     HH.modifies_rref tls_tables_region !{HH.as_ref (MR.as_rref conn_tab)} h0 h1 /\
+	     HH.contains_ref (MR.as_rref conn_tab) h1 /\
+	     (* HH.contains_ref (MR.as_rref MS.ms_tab) h0 /\ *)
 	     conn_hs_region_exists c h0 /\
 	     is_hs_rgn (HS.region c.hs) /\
-	     (let old_conn = MR.m_sel h0 conn_table in 
-    	      let new_conn = MR.m_sel h1 conn_table in 
+	     (let old_conn = MR.m_sel h0 conn_tab in 
+    	      let new_conn = MR.m_sel h1 conn_tab in 
 	      let nonce = I.nonce_of_id i in 
 	      MM.sel old_conn nonce = None /\
 	      new_conn = MM.upd old_conn nonce c)))
@@ -301,8 +346,8 @@ val add_connection_ok: h0:HH.t -> h1:HH.t -> i:id -> c:i_conn i -> Lemma
 let add_connection_ok h0 h1 i c = 
     let old_ms = MR.m_sel h0 MS.ms_tab in 
     let new_ms = MR.m_sel h1 MS.ms_tab in
-    let old_conn = MR.m_sel h0 conn_table in 
-    let new_conn = MR.m_sel h1 conn_table in
+    let old_conn = MR.m_sel h0 conn_tab in 
+    let new_conn = MR.m_sel h1 conn_tab in
     let hs_region_exists : n:random -> Lemma
     	(is_Some (MM.sel new_conn n) ==> conn_hs_region_exists (Some.v (MM.sel new_conn n)) h1) =
       fun n -> match MM.sel new_conn n with
